# Lambek Calculus

## Syntactic Rules

- **Rule 1**: "Simplification"
$$
(x/y)y \rightarrow x
$$
$$
y(y\backslash x) \rightarrow x
$$

- **Rule 2**: "V-Associativity"
$$
(x\backslash y)/z \leftrightarrows x\backslash (y/z)
$$

- **Rule 3**: "Elimination"
$$
(x/y)(y/z) \rightarrow x/z
$$
$$
(x\backslash y)(y\backslash z) \rightarrow x\backslash z
$$

- **Rule 4**: "Type Raising"
$$
x \rightarrow y/(x \backslash y)
$$
$$
x \rightarrow (y / x) \backslash x
$$

## Formal Definition

### Definitions

#### Foundational Notions

1. Let $X$ be a set of strings, called the *lexicon*. Elements of $X$ are called *lexemes*.
2. Let $X^+$ be the collection of all finite, non-empty lexeme sequences.
3. For all $A,B\in X^+$, where $A=\langle A_0, \ldots, A_n \rangle$ and $B=\langle B_0, \ldots, B_m \rangle$, define the *concatenation* $AB$ as the sequence $\langle A_0, \ldots, A_n, B_0, \ldots, B_m \rangle$.
4. Let $L\subseteq X^+$ be non-empty. $L$ is called the *language*. Elements of $L$ are called *sentences*.
5. Let $P$ be a non-empty set. Elements of $P$ are called *primitive types*.
6. Let $s\in P$ be called the "sentence type".
7. Let $T \supset P$. Elements of $T$ are called *types*, and they are either of the form $a$, $a/b$, $a\backslash b$, or $ab$ (or $\ a\cdot b$) where $a,b\in T$.
8. Let $\triangleright \in X^+\times T$. When $p \triangleright t$, we say $t$ is a *type* of $p$.
9. Let **LC** = $\langle X, L, T, P, \triangleright \rangle$. We call **LC** a *lambek calculus*.

#### (A) Arrow Relations

There is an implication relation $\rightarrow$ on types that connects the logic of the types to the structure of the language.

1. $\forall x,y \in T : x \rightarrow y \Leftrightarrow \forall A \in X^+: A \triangleright x \Rightarrow A \triangleright y$
2. $\forall x,y \in T : x \rightleftarrows y \Leftrightarrow x\rightarrow y \ \& \ y \rightarrow x$

#### Length Function

It is convenient to have a notion of "product length", i.e. how many times does the $\cdot$ operator occur in a type, or how many lexemes are there in a sentence.

1. Let $\mathtt{len}: X^{+}\ \cup\ T \rightarrow \mathbb{N}$, where:
   1. For all lexemes $W\in X$, define $\mathtt{len}(W) = 1$.
   2. For all lexeme sequences $A, B\in X^+$, define $\mathtt{len}(AB) = \mathtt{len}(A) + \mathtt{len}(B)$.
   3. For all types $x\in T$,
      1. If $x=y\cdot z$ for some $y,z\in T$ then $\mathtt{len}(x) = \mathtt{len}(y) + \mathtt{len}(z)$;
      2. Otherwise, $\mathtt{len}(x)=1$.

**Proof** that $\mathtt{len}$ is a well defined function:
- First, need to establish that $\mathtt{len}$ is well defined on $X^+$.
  - For all $W\in X$, $\mathtt{len}(W)=1$ by definition, and hence is well defined.
  - Suppose $\mathtt{len}$ is well defined on all $X^i$ where $i\leq n$ for some $n\in\mathbb{N}$.
    - Consider $A\in X^{n+1}$. Note that $A=A_0A_1\ldots A_n$.
    - Choose $m\in\mathbb{N}$ such that $0<m\leq n$.
    - Then $A=(A_0\ldots A_m)(A_{m+1}\ldots A_n)$.
    - Note that $(A_0\ldots A_m)\in X^{m+1}$ and $(A_{m+1}\ldots A_n)\in X^{n-m}$.
    - By inductive hypothesis, $\mathtt{len}$ is well defined on $X^{m+1}$ and $X^{n-m}$.
    - Since $\mathtt{len}(A) = \mathtt{len}(A_0\ldots A_m) + \mathtt{len}(A_{m+1}\ldots A_n)$ by definition, see that $\mathtt{len}$ is well defined on $X^{n+1}$.
- Then we need to establish the same for $T$.
  - Clearly true, lacking convenient notation for proof ...

### Axioms

#### (T) Type Axioms

1. Every primitive type is instantiated at least once in the lexicon.

   $\forall p\in P\ \exists W \in X: W\triangleright p$

2. Every lexeme has at least one type of length 1.

   $\forall W\in X\ \exists x\in T: \mathtt{len}(x)=1\ \&\ W\triangleright x$


#### (P) Product Axioms

For all lexeme sequences $A,B\in X^+$ and all types $x,y \in T$,

1. $A\triangleright xy \Rightarrow ( \exists C,D\in X^+ : A=CD\ \&\ C\triangleright x \ \&\ D \triangleright y)$
2. $A \triangleright x\ \& \ B\triangleright y \Rightarrow AB \triangleright xy$

#### (S) Slash Axioms

1. $\forall A \in X^+\ \forall y, z \in T : A \triangleright z/y \Leftrightarrow (\forall B \in X^+: B \triangleright y \Rightarrow AB \triangleright z)$
2. $\forall B \in X^+\ \forall x, z \in T :  B \triangleright x\backslash z \Leftrightarrow (\forall A \in X^+: A \triangleright x \Rightarrow AB \triangleright z)$

### Theorems

#### (L) Lemmas


1. Product typed lexeme sequences are never of length one. <!--Note, this can probably be strengthened to len(A)=n.-->

   $\forall A\in X^+\ \forall x,y \in T: A\triangleright xy \Rightarrow \mathtt{len}(A)>1$

   - **Proof**. Assume $A\triangleright xy$.
   - Then by (P1), $A=BC$ for some $B,C\in X^+$ where $B\triangleright x$ and $C\triangleright y$.
   - Hence $\mathtt{len}(A) = \mathtt{len}(B) + \mathtt{len}(C) \geq 2$.

2. All lexeme sequences of length $n$ have a type of length $n$.

   $\forall A\in X^+: \mathtt{len}(A)=n \Rightarrow \exists x\in T : \mathtt{len}(x)=n\ \&\ A\triangleright x$

   - **Proof** by induction on length.
   - Assume $\mathtt{len}(A)=1$.
     - Then $A\in X$ by definition of $\mathtt{len}$.
     - Hence by (T2), $A\triangleright x$ for some $x\in T$ where $\mathtt{len}(x)=1$.
   - Assume the theorem is true for $\mathtt{len}(A) = n$.
     - Let $A\in X^T$ be such that $\mathtt{len}(A)=n+1$.
     - Hence $A=A_0\cdots A_n=(A_0\cdots A_{n-1})\cdot A_n$.
     - By inductive hypothesis, $(A_0\cdots A_{n-1}) \triangleright x$ for some $x\in T$ such that $\mathtt{len}(x)=n$.
     - By (T2), $A_n \triangleright y$ for some $y\in T$ where $\mathtt{len}(x)=1$.
     - Hence $A=(A_0\cdots A_{n-1})\cdot A_n\triangleright xy$ by (P2).
     - By definition, $\mathtt{len}(xy)=\mathtt{len}(x)+\mathtt{len}(y)=n+1$.

3. All lexeme sequences have at least one type.

   $\forall A \in X^+\ \exists x \in T: A \triangleright x$.

   - **Proof**. Follows immediately from (L2).

#### Lambek's Theorems

1. $\forall x \in T: x \rightarrow x$
   - **Proof**. Note that, by (A1), $x \rightarrow x \Leftrightarrow \forall A \in L: A \triangleright x \Rightarrow A \triangleright x$.
   - This is true since $p\Rightarrow p$ is true for any proposition $p$.

2. $\forall x, y, z \in T: x(yz) \rightleftarrows (xy)z$
   - **Proof**. $(\rightarrow)$
     - By (A1), $x(yz) \rightarrow (xy)z$ if and only if $\forall A \in L: A \triangleright x(yz) \Rightarrow A \triangleright (xy)z$.
     - Suppose $A \triangleright x(yz)$. Then by (P1), $A=BC$ for some $B,C$ where $B\triangleright x$ and $C \triangleright yz$.
     - Again by (P1), get that $C=DE$ for some $D,E$ where $D\triangleright y$ and $E \triangleright z$.
     - Since $C=DE$ and $C\triangleright yz$, conclude $DE\triangleright yz$.
     - By (P2), conclude that $D\triangleright y$ and $E\triangleright z$.
     - $A = BDE$ has been established. Since concatenation is associative, $BDE = B(DE)$.
     - Since $A \triangleright x(yz)$, conclude $B(DE) \triangleright x(yz)$. By (P2), $B \triangleright x$.
     - Since $B \triangleright x$ and $D \triangleright y$, conclude $BD\triangleright xy$ by (P2).
     - Again by (P2), conclude $(BD)E \triangleright (xy)z$.
     - Since $A=B(DE)=(BD)E$, conclude $A\triangleright (xy)z$.
   - Now we prove ($\leftarrow$).
     - By (A1), $(xy)z \rightarrow x(yz)$ if and only if $\forall A \in L: A \triangleright (xy)z \Rightarrow A \triangleright x(yz)$.
     - Suppose $A \triangleright (xy)z$. Then by (P1), $A=BC$ for some $B,C$ where $B\triangleright (xy)$ and $C \triangleright z$.
     - Again by (P1), get that $B=DE$ for some $D,E$ where $D\triangleright x$ and $E \triangleright y$.
     - Since $B=DE$ and $B\triangleright xy$, conclude $DE\triangleright xy$.
     - By (P2), conclude that $D\triangleright x$ and $E\triangleright y$.
     - $A = DEC$ has been established. Since concatenation is associative, $DEC = (DE)C$.
     - Since $A \triangleright (xy)z$, conclude $(DE)C \triangleright (xy)z$. By (P2), $C \triangleright z$.
     - Since $E \triangleright y$ and $C \triangleright z$, conclude $EC\triangleright yz$ by (P2).
     - Again by (P2), conclude $D(EC) \triangleright x(yz)$.
     - Since $A=(DE)C=D(EC)$, conclude $A\triangleright x(yz)$.

3. $\forall x, y, z \in T: xy \rightarrow z \Leftrightarrow x \rightarrow z/y$
  - **Proof**. $(\Rightarrow)$
    - Assume $xy \rightarrow z$.
    - Let $A\triangleright x$ and $B\triangleright y$.
    - Then $AB\triangleright xy$ by (P2).
    - Hence $AB\triangleright z$ by (A1).
    - Since $B\triangleright y$ and $AB\triangleright z$, conclude $A\triangleright z/y$ by (S1).
    - Hence $x\rightarrow z/y$.
  - Now we prove ($\Leftarrow$).
    - Assume $x\rightarrow z/y$.
    - Let $A\triangleright xy$.
    - By (P1), $A=BC$ for some $B,C$ such that $B\triangleright x$ and $C\triangleright y$.
    - Since $x\rightarrow z/y$, conclude $B\triangleright z/y$ by (A1).
    - Since $B\triangleright z/y$ and $C\triangleright y$, conclude $BC\triangleright z$ by (S1).
    - Since $A=BC$, conclude $A\triangleright z$.
    - Hence $xy\rightarrow z$.

4. $\forall x, y \in T: xy \rightarrow z \Leftrightarrow y \rightarrow x\backslash z$
  - **Proof**. $(\Rightarrow)$
    - Assume $xy \rightarrow z$.
    - Let $A\triangleright x$ and $B\triangleright y$.
    - Then $AB\triangleright xy$ by (P2).
    - Hence $AB\triangleright z$ by (A1).
    - Since $A\triangleright x$ and $AB\triangleright z$, conclude $B\triangleright x\backslash z$ by (S2).
    - Hence $y\rightarrow x\backslash z$.
  - Now we prove ($\Leftarrow$).
    - Assume $y\rightarrow x\backslash z$.
    - Let $A\triangleright xy$.
    - By (P1), $A=BC$ for some $B,C$ such that $B\triangleright x$ and $C\triangleright y$.
    - Since $x\rightarrow x\backslash z$, conclude $C\triangleright x\backslash z$ by (A1).
    - Since $C\triangleright x\backslash z$ and $B\triangleright x$, conclude $BC\triangleright z$ by (S2).
    - Since $A=BC$, conclude $A\triangleright z$.
    - Hence $xy\rightarrow z$.

5. $\forall x, y \in T: x\rightarrow y \ \&\ y\rightarrow z \Rightarrow x \rightarrow z$
  - **Proof**.
    - stub


## References
- "The Mathematics of Sentence Structure" by Joachim Lambek, 1958
